

Chukwuemeka Ajaero, 8593168

### Exercise 1

$\langle \text{program} \rangle \rightarrow \text{begin } \langle \text{statement\_list} \rangle \text{ end}$   
 $\langle \text{statement\_list} \rangle \rightarrow \langle \text{statement} \rangle ; \langle \text{statement\_list} \rangle$   
 $\langle \text{statement\_list} \rangle \rightarrow \langle \text{statement} \rangle$   
 $\langle \text{statement} \rangle \rightarrow \text{id} = \langle \text{expression} \rangle$   
 $\langle \text{expression} \rangle \rightarrow \langle \text{factor} \rangle + \langle \text{factor} \rangle$   
 $\langle \text{expression} \rangle \rightarrow \langle \text{factor} \rangle - \langle \text{factor} \rangle$   
 $\langle \text{expression} \rangle \rightarrow \langle \text{factor} \rangle$   
 $\langle \text{factor} \rangle \rightarrow \text{id} \mid \text{num}$

#### ① Eliminating Left recursion

The grammar does not contain left recursion as none of the grammar fragments are in the form  $A \rightarrow A\alpha \mid \beta$ .

#### ② Left factoring

After left factoring, you get the following grammar

$\langle \text{program} \rangle \rightarrow \text{begin } \langle \text{statement\_list} \rangle \text{ end}$   
 $\langle \text{statement\_list} \rangle \rightarrow \langle \text{statement} \rangle \langle \text{statement\_list}' \rangle$   
 $\langle \text{statement\_list}' \rangle \rightarrow ; \langle \text{statement\_list} \rangle \mid \epsilon$   
 $\langle \text{statement} \rangle \rightarrow \text{id} = \langle \text{expression} \rangle$   
 $\langle \text{expression} \rangle \rightarrow \langle \text{factor} \rangle \langle \text{expression}' \rangle$   
 $\langle \text{expression}' \rangle \rightarrow + \langle \text{factor} \rangle \mid - \langle \text{factor} \rangle \mid \epsilon$   
 $\langle \text{factor} \rangle \rightarrow \text{id} \mid \text{num}$

Chukwuemeka Ajaero, 8593168

### Exercise 3

- ①
- $\langle \text{program} \rangle \rightarrow \text{begin } \langle \text{statement\_list} \rangle \text{ end}$
  - $\langle \text{statement\_list} \rangle \rightarrow \langle \text{statement} \rangle \langle \text{statement\_list}' \rangle$
  - $\langle \text{statement\_list}' \rangle \rightarrow ; \langle \text{statement\_list} \rangle \mid \epsilon$
  - $\langle \text{statement} \rangle \rightarrow \text{id} = \langle \text{expression} \rangle$
  - $\langle \text{expression} \rangle \rightarrow \langle \text{factor} \rangle \langle \text{expression}' \rangle$
  - $\langle \text{expression}' \rangle \rightarrow + \langle \text{factor} \rangle \mid - \langle \text{factor} \rangle \mid \epsilon$
  - $\langle \text{factor} \rangle \rightarrow \text{id} \mid \text{num}$

- \*  $\text{FIRST}(\text{program}) = \{ \text{begin} \}$
- \*  $\text{FIRST}(\text{statement\_list}) = \{ \text{FIRST}(\text{statement}) \} = \{ \text{id}, = \}$
- \*  $\text{FIRST}(\text{statement\_list}') = \{ ;, \epsilon \}$  Need to ask whether this should be one terminal or two
- \*  $\text{FIRST}(\text{statement}) = \{ \text{id}, = \}$  ←
- \*  $\text{FIRST}(\text{expression}) = \{ \text{FIRST}(\text{factor}) \} = \{ \text{id}, \text{num} \}$
- \*  $\text{FIRST}(\text{expression}') = \{ +, -, \epsilon \}$
- \*  $\text{FIRST}(\text{factor}) = \{ \text{id}, \text{num} \}$
- \*  $\text{FOLLOW}(\text{program}) = \{ \$ \}$
- \*  $\text{FOLLOW}(\text{statement\_list}) = \{ \text{end}, \text{FOLLOW}(\text{statement\_list}') \}$   
 $= \{ \text{end} \}$  Asked the prof about what to do in this situation. Waiting for a response.
- \*  $\text{FOLLOW}(\text{statement\_list}') = \{ \text{FOLLOW}(\text{statement\_list}) \}$   
 $= \{ \text{end} \}$
- \*  $\text{FOLLOW}(\text{statement}) = \{ (\text{FIRST}(\text{statement\_list}') - \epsilon) \cup \text{FOLLOW}(\text{statement\_list}') \}$   
 $= \{ ;, \text{end} \}$  ←

Chukwuemeka Ajaero, 8593168

- \*  $\text{FOLLOW}(\text{expression}) = \{ \text{FOLLOW}(\text{statement}) \}$   
 $= \{ ;, \text{end} \}$  ← Remember to redo if wrong
- \*  $\text{FOLLOW}(\text{expression}') = \{ \text{FOLLOW}(\text{expression}) \}$   
 $= \{ ;, \text{end} \}$  ←
- \*  $\text{FOLLOW}(\text{factor}) = \{ (\text{FIRST}(\text{expression}') - \epsilon) \cup$   
 $\text{FOLLOW}(\text{expression}), \text{FOLLOW}(\text{expression}') \}$   
 $= \{ +, -, *, /, \text{end} \}$  ← Redo

**Exercise 3.2**

	begin	end	;	id	num	=	+	-	\$
program	<program > → begin <statemen t_list> end	-	-	-	-	-	-	-	-
statement _list	-	-	-	<statemen t_list> → <statemen t> <statemen t_list'>	-	<statemen t_list> → <statemen t> <statemen t_list'>	-	-	-
statement _list'	-	<statemen t_list'> → $\epsilon$	<statemen t_list'> → ; <statemen t_list>	-	-	-	-	-	-
statement	-	-	-	<statemen t> id = <expressi on>	-	<statemen t> id = <expressi on>	-	-	-
expression	-	-	-	<expressi on> → <factor> <expressi on'>	<expressi on> → <factor> <expressi on'>	-	-	-	-
expression ,	-	<expressi on> → $\epsilon$	<expressi on> → $\epsilon$	-	-	-	<expressi on> →	<expressi on> →	-

							+<factor>	-<factor>	
factor	-	-	-	<factor> → id	<factor> → num	-	-	-	-